code/salsa-family/Hacl.Test.Chacha20.fst
@@ -1,14 +1,14 @@
 module Hacl.Test.Chacha20
 
-open Hacl.Symmetric.Chacha20
 open FStar.Buffer
+module Chacha20=Hacl.Symmetric.Chacha20
 
 let len = 114ul
 
 #set-options "--initial_fuel 0 --max_fuel 0 --z3rlimit 20"
 
 private let rec loop
-  (st:chacha_ctx)
+  (st:Chacha20.chacha_ctx)
   (c:buffer UInt8.t{disjoint st c})
   (m:buffer UInt8.t)
   (len:UInt32.t{length c >= UInt32.v len /\ length m >= UInt32.v len})
@@ -16,7 +16,7 @@ private let rec loop
                (ensures (fun h0 _ h1 -> live h1 st /\ live h1 c /\ live h1 m /\ modifies_2 st c h0 h1))
   = if FStar.UInt32.(len <^ 64ul) then ()
     else (
-      chacha20_update st (sub m 0ul 64ul) (sub c 0ul 64ul);
+      Chacha20.chacha20_update st (sub m 0ul 64ul) (sub c 0ul 64ul);
       loop st (offset c 64ul) (offset m 64ul) FStar.UInt32.(len -^ 64ul)
     )
 
@@ -72,15 +72,15 @@ let main () =
     ] in
   let counter = 1ul in
   let ctx = create 0ul 32ul in
-  Hacl.Symmetric.Chacha20.chacha_keysetup ctx key;
-  Hacl.Symmetric.Chacha20.chacha_ietf_ivsetup ctx nonce counter;
-  Hacl.Symmetric.Chacha20.chacha_encrypt_bytes ctx plaintext ciphertext len;
+  Chacha20.chacha_keysetup ctx key;
+  Chacha20.chacha_ietf_ivsetup ctx nonce counter;
+  Chacha20.chacha_encrypt_bytes ctx plaintext ciphertext len;
   TestLib.compare_and_print (C.string_of_literal "chacha20") expected ciphertext len;
-  let ctx = chacha20_init key nonce counter in
+  let ctx = Chacha20.chacha20_init key nonce counter in
   loop ctx ciphertext plaintext len;
   let r = FStar.UInt32.(len &^ 0x3ful) in
   let q = FStar.UInt32.(len >>^ 6ul) in
-  chacha20_finish ctx (Buffer.offset plaintext FStar.UInt32.(q *^ 64ul))
+  Chacha20.chacha20_finish ctx (Buffer.offset plaintext FStar.UInt32.(q *^ 64ul))
                       (Buffer.offset ciphertext FStar.UInt32.(q *^ 64ul)) r;
   TestLib.compare_and_print (C.string_of_literal "chacha20") expected ciphertext len;
   pop_frame();
